\title{Tittel.}
\author{Magne Tenstad}
\date{Oktober 23}

\begin{document}
	\begin{align*}
		g\left(x\right)&= \left(x^2+2\cdot x+\frac{2}{\left(x+1\right)}+2\right)\\
		g\left(1\right)&= \left(1^2+2\cdot 1+\frac{2}{\left(1+1\right)}+2\right)\\
		&= 6.0\\
		g\left(g\left(x\right)\right)&= \left(\left(x^2+2\cdot x+\frac{2}{\left(x+1\right)}+2\right)^2+2\cdot \left(x^2+2\cdot x+\frac{2}{\left(x+1\right)}+2\right)+\frac{2}{\left(\left(x^2+2\cdot x+\frac{2}{\left(x+1\right)}+2\right)+1\right)}+2\right)\\
		g\left(g\left(1\right)\right)&= \left(\left(1^2+2\cdot 1+\frac{2}{\left(1+1\right)}+2\right)^2+2\cdot \left(1^2+2\cdot 1+\frac{2}{\left(1+1\right)}+2\right)+\frac{2}{\left(\left(1^2+2\cdot 1+\frac{2}{\left(1+1\right)}+2\right)+1\right)}+2\right)\\
		&= 50.29\\
	\end{align*}
\end{document}
